Pack.v: use a Section instead of a Module
using a Module required the use of another module to pass in
the expected item size, which in turn made the item size too
opaque for the caller of Pack.v to manipulate.

src/Pack.v
@@ -3,43 +3,40 @@ Require Import Prog.
 Require Import Arith.
 Require Import Eqdep.
 
+Set Implicit Arguments.
 
-Module Type ItemSize.
-  Parameter itemsz : nat.
-  Parameter items_per_valu : addr.
-  Axiom itemsz_ok : wordToNat items_per_valu * itemsz = valulen.
-  (* This is in lieu of actually being able to do division.. *)
-End ItemSize.
+Section Packer.
+  Variable itemsz : nat.
+  Variable items_per_valu : addr.
+  Variable itemsz_ok : wordToNat items_per_valu * itemsz = valulen.
 
-
-Module Packer (IS: ItemSize).
-  Theorem extract_len : forall pos, (pos < IS.items_per_valu)%word
-    -> wordToNat pos * IS.itemsz + IS.itemsz + (valulen - wordToNat pos * IS.itemsz - IS.itemsz)
+  Theorem extract_len : forall pos, (pos < items_per_valu)%word
+    -> wordToNat pos * itemsz + itemsz + (valulen - wordToNat pos * itemsz - itemsz)
        = valulen.
   Proof.
     intros pos H. rewrite <- Nat.sub_add_distr. rewrite le_plus_minus_r.
-    reflexivity. rewrite <- Nat.mul_succ_l. rewrite <- IS.itemsz_ok.
+    reflexivity. rewrite <- Nat.mul_succ_l. rewrite <- itemsz_ok.
     apply mult_le_compat_r. apply Nat.le_succ_l. apply wlt_lt. assumption.
   Qed.
 
-  Definition extract (v : valu) (pos : addr) : word IS.itemsz.
-    refine (if wlt_dec pos IS.items_per_valu then _ else wzero IS.itemsz).
-    refine (let below := (wordToNat pos) * IS.itemsz in _).
-    refine (let above := valulen - below - IS.itemsz in _).
+  Definition extract (v : valu) (pos : addr) : word itemsz.
+    refine (if wlt_dec pos items_per_valu then _ else wzero itemsz).
+    refine (let below := (wordToNat pos) * itemsz in _).
+    refine (let above := valulen - below - itemsz in _).
     erewrite <- extract_len in v by eassumption.
-    refine (let v_lower := split1 (below + IS.itemsz) above v in _).
-    refine (let result := split2 below IS.itemsz v_lower in _).
+    refine (let v_lower := split1 (below + itemsz) above v in _).
+    refine (let result := split2 below itemsz v_lower in _).
     exact result.
   Defined.
 
-  Definition update (v : valu) (pos : addr) (n : word IS.itemsz) : valu.
-    refine (if wlt_dec pos IS.items_per_valu then _ else v).
-    refine (let below := (wordToNat pos) * IS.itemsz in _).
-    refine (let above := valulen - below - IS.itemsz in _).
+  Definition update (v : valu) (pos : addr) (n : word itemsz) : valu.
+    refine (if wlt_dec pos items_per_valu then _ else v).
+    refine (let below := (wordToNat pos) * itemsz in _).
+    refine (let above := valulen - below - itemsz in _).
     erewrite <- extract_len in v by eassumption.
-    refine (let v_above := split2 (below + IS.itemsz) above v in _).
-    refine (let v_lower := split1 (below + IS.itemsz) above v in _).
-    refine (let v_below := split1 below IS.itemsz v_lower in _).
+    refine (let v_above := split2 (below + itemsz) above v in _).
+    refine (let v_lower := split1 (below + itemsz) above v in _).
+    refine (let v_below := split1 below itemsz v_lower in _).
     refine (let result := combine (combine v_below n) v_above in _).
     subst below; subst above.
     rewrite extract_len in result by eassumption.
@@ -49,31 +46,31 @@ Module Packer (IS: ItemSize).
   (* extract' and update' avoid rewriting types, so they have no eq_rect terms,
    * but instead they have dependent matches..  unclear which is worse.
    *)
-  Definition extract' (v : valu) (pos : addr) : word IS.itemsz.
-    refine (if wlt_dec pos IS.items_per_valu then _ else wzero IS.itemsz).
-    refine (let below := (wordToNat pos) * IS.itemsz in _).
-    refine (let above := valulen - below - IS.itemsz in _).
-    refine (let v' := match (eq_sym (extract_len pos w)) in _ = N return word N with
+  Definition extract' (v : valu) (pos : addr) : word itemsz.
+    refine (if wlt_dec pos items_per_valu then _ else wzero itemsz).
+    refine (let below := (wordToNat pos) * itemsz in _).
+    refine (let above := valulen - below - itemsz in _).
+    refine (let v' := match (eq_sym (extract_len w)) in _ = N return word N with
                       | refl_equal => v
                       end in _).
-    refine (let v_lower := split1 (below + IS.itemsz) above v' in _).
-    refine (let result := split2 below IS.itemsz v_lower in _).
+    refine (let v_lower := split1 (below + itemsz) above v' in _).
+    refine (let result := split2 below itemsz v_lower in _).
     exact result.
   Defined.
 
-  Definition update' (v : valu) (pos : addr) (n : word IS.itemsz) : valu.
-    refine (if wlt_dec pos IS.items_per_valu then _ else v).
-    refine (let below := (wordToNat pos) * IS.itemsz in _).
-    refine (let above := valulen - below - IS.itemsz in _).
-    refine (let v' := match (eq_sym (extract_len pos w)) in _ = N return word N with
+  Definition update' (v : valu) (pos : addr) (n : word itemsz) : valu.
+    refine (if wlt_dec pos items_per_valu then _ else v).
+    refine (let below := (wordToNat pos) * itemsz in _).
+    refine (let above := valulen - below - itemsz in _).
+    refine (let v' := match (eq_sym (extract_len w)) in _ = N return word N with
                       | refl_equal => v
                       end in _).
-    refine (let v_above := split2 (below + IS.itemsz) above v' in _).
-    refine (let v_lower := split1 (below + IS.itemsz) above v' in _).
-    refine (let v_below := split1 below IS.itemsz v_lower in _).
+    refine (let v_above := split2 (below + itemsz) above v' in _).
+    refine (let v_lower := split1 (below + itemsz) above v' in _).
+    refine (let v_below := split1 below itemsz v_lower in _).
     refine (let result := combine (combine v_below n) v_above in _).
     subst below; subst above.
-    refine (let result' := match (extract_len pos w) in _ = N return word N with
+    refine (let result' := match (extract_len w) in _ = N return word N with
                            | refl_equal => result
                            end in _).
     exact result'.
@@ -91,12 +88,12 @@ Module Packer (IS: ItemSize).
   Qed.
 
   Theorem extract_same : forall v pos pos' n, pos = pos'
-    -> (pos < IS.items_per_valu)%word
+    -> (pos < items_per_valu)%word
     -> extract (update v pos' n) pos = n.
   Proof.
     intros; subst pos'.
     unfold extract, update.
-    destruct (wlt_dec pos IS.items_per_valu); try congruence.
+    destruct (wlt_dec pos items_per_valu); try congruence.
 
     unfold eq_rec_r, eq_rec.
     repeat rewrite eq_rect_double.
@@ -112,8 +109,8 @@ Module Packer (IS: ItemSize).
   Proof.
     intros.
     unfold extract, update.
-    destruct (wlt_dec pos IS.items_per_valu); auto.
-    destruct (wlt_dec pos' IS.items_per_valu); auto.
+    destruct (wlt_dec pos items_per_valu); auto.
+    destruct (wlt_dec pos' items_per_valu); auto.
 
     unfold eq_rec_r, eq_rec.
     repeat rewrite eq_rect_double.
